Add files via upload
hamt implementation with comments

HAMT.v
@@ -1,4 +1,5 @@
 (* Notation *)
+(* These are just declaring to Coq common notation I will be using throughout the project *)
 
 Notation "( x , y )" := (pair x y).
 Notation "X * Y" := (prod X Y) : type_scope.
@@ -10,6 +11,7 @@ Notation "[ x ; .. ; y ]" := (cons x .. (cons y nil) ..).
 Definition mylist := 1 :: (2 :: (3 :: nil)).
 
 (* Imports *)
+(* Common modules I will be using throughout the implementation *)
 
 Require Coq.extraction.Extraction.
 Extraction Language OCaml.
@@ -24,6 +26,7 @@ From Coq Require Import ZArith.Znat.
 
 (* Definitions *)
 
+(* Function that takes two natural numbers and returns a boolean describing their equality *)
 Fixpoint eqb (n m : nat) : bool :=
   match n with
   | O => match m with
@@ -36,9 +39,13 @@ Fixpoint eqb (n m : nat) : bool :=
             end
   end.
 
+(* keys are defined as nats in this implementation *)
 Definition key := nat.
+(* shift value used for indexing into the arrays using bits of the hash *)
 Definition shift :Z := 5. 
+(* mask out everything but the first 5 bits *)
 Definition mask :Z := 31.
+(* Following two numbers are used for the hashing function, taken from the Fowler–Noll–Vo hash function *)
 Definition FMV_prime : Z := 1099511628211.
 Definition FMV_offset : Z := 14695981039346656037.
 
@@ -46,15 +53,20 @@ Definition FMV_offset : Z := 14695981039346656037.
 
 Module HAMT.
 
+(* Inductively define HAMT as an empty node, a hashmap entry which hols a key val pair, collision node if 
+two keys hash to the same integer, and array node that holds more HAMT's *)
+(* Takes a type that is the type of the value *)
 Inductive HAMT (A : Type) : Type :=
   | Empty
   | HashMapEntry (hash : Z) (k : key) (val : A)
   | ArrayNode (shift : Z) (map : array (HAMT A))
   | CollisionNode (hash : Z) (hmes : list (key * A)).
   
+(* Function that takes a value type and returns an Empty HAMT of that type *)
 Definition empty_HAMT (A:Type) : HAMT A :=
     Empty A.
 
+(* hash function that copies the Fowler-Noll-Vo hash function *)
 Definition hasher2 (key : nat) : Z := 
         let hash := FMV_offset in
         let int_initial := Z.of_nat key in 
@@ -75,7 +87,8 @@ Definition hasher2 (key : nat) : Z :=
         let hash := Z.mul FMV_prime hash in 
         let hash := Z.lor hash (Z.land int_initial 18374686479671623680) in
         hash. 
-    
+
+(* iterates through list of key value pairs and returns an option, used as a helper function for find *)
 Fixpoint findv (A : Type) (hmes : list (key * A)) (k1 : key) :=
   match hmes with 
   |[] => None
@@ -83,55 +96,70 @@ Fixpoint findv (A : Type) (hmes : list (key * A)) (k1 : key) :=
     if (eqb k k1) then Some v else findv A t k1
   end.
 
+(* Funnction that takes a type, hamt, key, and returns the value associated with that key if it is in the HAMT *)
 Fixpoint find (A : Type) (hamt : HAMT A) (k : key) : option A :=
   match hamt with 
   |HashMapEntry _ hash k1 val  => 
       if eqb k k1 then Some val else None
   | ArrayNode _ shift map => 
+      (* if the HAMT is an array node, need to use the hashed key to index into the array, at the correct depth *)
       find A (get map (of_Z(Z.land (Z.shiftr (hasher2 k) shift) mask))) k
   | CollisionNode _ hash hmes => 
+      (* call helper function *)
       findv A hmes k
   | Empty _ => 
       None
   end.
 
+(* helper function for the remove function, iterates through collisionNode list and removes key val pair *)
 Fixpoint remove_ass (A : Type) (k : key) (l : list (key * A)) : list (key * A) :=
     match l with
     | nil => nil
     | (k1, v) :: tl => if (eqb k k1) then remove_ass A k tl else (k1, v) :: (remove_ass A k tl)
     end.
-       
+    
+(* Function that takes a hamt and removes a key val pair, returning an empty HAMT in place of the hash map entry *)
 Fixpoint remove (A : Type) (hamt : HAMT A) (k : key) : HAMT A :=
    match hamt with 
+   (* if the hamt is an ArrayNode, we need to index into the array using the hashed key and recursively call remove *)
    | ArrayNode _ shifter map => 
      let index := (of_Z(Z.land (Z.shiftr (hasher2 k) shifter) mask)) in 
      let newArr := copy map in 
      let newVal := remove A (get map index) k in 
      ArrayNode A shift (set map index newVal)
    | Empty _ => 
+      (* if we reach an Empty hash, we know the key is not in the hash and we can just return an empty hamt *)
        Empty A
    | CollisionNode _ hash hmes => 
+       (* if we reach a collision node, send the list to the helper function *)
        let newl := (remove_ass A k hmes) in 
        match newl with 
        |[] => Empty A
        |_ :: _ => CollisionNode A hash newl
        end
    | HashMapEntry _ hash1 key val1 => 
+       (* if we find the entry, return an empty hash in its place *)
        Empty A
    end.
 
+(* function to add a key val pair to the hamt *)
 Fixpoint add (A : Type) (hamt : HAMT A) (k : key) (val : A) (shifter : Z) : HAMT A :=
     match hamt with 
     | ArrayNode _ shift1 map => 
+      (* if we find an ArrayNode, we need to index into that array using the hashed key, and recursively call add *)
       let index := (of_Z(Z.land (Z.shiftr (hasher2 k) shift1) mask)) in
       let newArr := copy map in 
       let newVal := add A (get map index) k val (shifter + shift) in 
       ArrayNode A shift1 (set map index newVal)
     | Empty _ => 
+      (* once we find an empty hamt, we can insert a hashmapentry holding the key val pair *)
       HashMapEntry A (hasher2 k) k val
     | CollisionNode _ hash hmes => 
+      (* if we have already had a collision at this hash, add to the collision list the key val pair *)
       CollisionNode A hash ((k, val) :: hmes)
     | HashMapEntry _ hash1 key val1 => 
+      (* if we collide with another hash, then get the index of each key, test to see if they are equal (if so make a 
+      collision node), and then create an ArrayNode holding each hashmapentry *)
       let index1 := (of_Z(Z.land (Z.shiftr (hasher2 key) shifter) mask)) in 
       let index2 := (of_Z(Z.land (Z.shiftr (hasher2 k) shifter) mask)) in
       let newArr := make 32 (empty_HAMT A) in 
@@ -144,32 +172,49 @@ Fixpoint add (A : Type) (hamt : HAMT A) (k : key) (val : A) (shifter : Z) : HAMT
 
 (* Correctness Axioms to Prove *)
 
+(* axiom stating that a find command on any key for an empty hamt returns non *)
 Axiom get_empty_default : forall (k : key) (A: Type),
       find A (empty_HAMT A) k = None.
-      
+
+(* axiom stating that a hamt always returns the key that has been added to the structure *)
 Axiom get_set_same : forall (A: Type) (k : key) (v : A) (hamt : HAMT A),
       find A (add A hamt k v 0) k = Some v.
        
+(* axiom stating that if two keys are not the same, adding one key doesn't disrupt the finding of another key *)
 Axiom get_set_other : forall (A: Type) (k k' : key) (v : A) (hamt : HAMT A),
      not (eq k k') -> find A (add A hamt k v 0) k' = find A hamt k'.
 
 (* Correctness Proof Theorems *)
 
+(* completed theorem resolving axiom 1 *)
 Theorem get_empty_default1: forall (A: Type) (k : key),
       find A (empty_HAMT A) k = None. 
   Proof.
   intros. unfold find. simpl. reflexivity.
 Qed.
 
+(* Incomplete theorem for axiom 2 *)
 Theorem get_set_same': forall (A: Type) (k : key) (v : A) (hamt : HAMT A),
       find A (add A hamt k v 0) k = Some v.
    Proof. Admitted.
    
+(* Incomplete theorem for axiom 3 *)
 Theorem get_set_other' : forall (A: Type) (k k' : key) (v : A) (hamt : HAMT A),
 not (eq k k') -> find A (add A hamt k v 0) k' = find A hamt k'.
     Proof. Admitted.
     
 (* Efficiency Proofs (Next Phase of Work)*)
+
+(* Extraction for Benchmarking *)
+
+Require Coq.extraction.Extraction.
+Extraction Language OCaml.
+
+(* Extract hashing function and dependencies *)
+Extraction "hamt_hash" hasher2 FMV_offset FMV_prime mask. 
+
+(* Extract hamt data structure and dependencies *)
+Extraction "hamt_bench" HAMT add remove find hasher2 empty_HAMT. 
 
 
   
